restructured, again

TypedAssembly/SystemF/Typ.lean
@@ -1,23 +1,50 @@
-inductive Typ : Nat → Type where
-  | var     : (x : Fin n) → Typ n
-  | int     : Typ n
-  | arrow   : Typ n → Typ n → Typ n
-  | prod    : Typ n → Typ n → Typ n
-  | for_all : Typ (n + 1) → Typ n
+import «TypedAssembly».SystemF.Kind
+
+inductive Ctxt where
+  | nil 
+  | cons : Ctxt → Kind → Ctxt
+  deriving BEq, DecidableEq, Repr
+
+namespace Ctxt 
+  notation "Ø" => Ctxt.nil
+  infixl:100 " ,⋆ " => Ctxt.cons
+end Ctxt
+open Ctxt
+
+
+inductive Lookupt : Ctxt → Kind → Type where
+  | here {Δ j} : Lookupt (Δ ,⋆ j) j
+  | there {Δ j k} : Lookupt Δ j → Lookupt (Δ ,⋆ k) j
+  deriving BEq, DecidableEq, Repr
+
+namespace Lookupt 
+  infixl:90 " ∋⋆ " => Lookupt
+end Lookupt
+open Lookupt
+
+inductive Typ   : Ctxt → Kind → Type where
+  | var {j}     : Δ ∋⋆ j → Typ Δ j
+  | int         : Typ Δ ⋆
+  | arrow       : Typ Δ ⋆ → Typ Δ ⋆ → Typ Δ ⋆
+  | prod        : Typ Δ ⋆ → Typ Δ ⋆ → Typ Δ ⋆
+  | for_all {j} : Typ (Δ ,⋆ j) ⋆ → Typ Δ ⋆
   deriving BEq, DecidableEq, Repr
 
 namespace Typ
-  postfix:90 " ⊢⋆ " => Typ
-  prefix:max " ♯ " => Typ.var
-  example : Typ 10 := ♯2
+  infixl:90 " ⊢⋆ " => Typ
+  syntax "♯" term : term
+  syntax "get_elem" (ppSpace term) : tactic
+  macro_rules | `(tactic| get_elem $n) => match n.1.toNat with
+  | 0 => `(tactic | exact Lookupt.here)
+  | n+1 => `(tactic| apply Lookupt.there; get_elem $(Lean.quote n))
 
   declare_syntax_cat typ
   syntax "!" term:max : typ
-  syntax:10 "∀. " typ : typ
-  syntax:50 typ (" → " <|> " -> ") typ : typ
-  syntax:50 typ " × " typ : typ
   syntax:90 "♯" num : typ
   syntax " int " : typ
+  syntax:50 typ (" → " <|> " -> ") typ : typ
+  syntax:50 typ " × " typ : typ
+  syntax:10 "∀. " typ : typ
   syntax " ⋆⟪ " typ " ⟫ " : term
 
   syntax " ( " typ " ) " : typ
@@ -25,84 +52,271 @@ namespace Typ
   macro_rules 
   | `( ⋆⟪ !$t ⟫) => `($t)
   | `( ⋆⟪ int ⟫ ) => `(Typ.int)
-  | `( ⋆⟪ ♯$n ⟫ ) => `(♯$n)
-  | `( ⋆⟪ $t₁:typ → $t₂:typ ⟫ ) => `(Typ.arrow ⋆⟪ $t₁ ⟫ ⋆⟪ $t₂ ⟫)
-  | `( ⋆⟪ $t₁:typ × $t₂:typ ⟫ ) => `(Typ.prod ⋆⟪ $t₁ ⟫ ⋆⟪ $t₂ ⟫)
-  | `( ⋆⟪ ∀. $t:typ ⟫) => `(Typ.for_all ⋆⟪ $t ⟫)
+  | `( ⋆⟪ ♯$n ⟫ ) => `(Typ.var (by get_elem $n))
+  | `( ⋆⟪ $t₁ → $t₂ ⟫ ) => `(Typ.arrow ⋆⟪ $t₁ ⟫ ⋆⟪ $t₂ ⟫)
+  | `( ⋆⟪ $t₁ × $t₂ ⟫ ) => `(Typ.prod ⋆⟪ $t₁ ⟫ ⋆⟪ $t₂ ⟫)
+  | `( ⋆⟪ ∀. $t ⟫) => `(Typ.for_all ⋆⟪ $t ⟫)
   | `( ⋆⟪ ( $t )  ⟫ ) => `(⋆⟪ $t ⟫)
 
-  def polyidt : n ⊢⋆ := ⋆⟪ ∀. ♯0 → ♯0 ⟫
+  example : Ø ,⋆ ⋆ ,⋆ ⋆ ,⋆ ⋆ ⊢⋆ ⋆ := ⋆⟪ ♯2 ⟫
+  def polyidt : Δ ⊢⋆ ⋆ := ⋆⟪ ∀. ♯0 → ♯0 ⟫
 
 end Typ
 open Typ
 
-@[simp, reducible] def liftTT (d : Nat) : n ⊢⋆ → (n + 1) ⊢⋆
-  | .var ix => 
-    if d <= ix then
-      (.var (ix.succ))
-    else .var (Fin.ofNat ix.val)
-  | .int => .int
-  | .arrow t₁ t₂ => .arrow (liftTT d t₁) (liftTT d t₂)
-  | .prod t₁ t₂ => .prod (liftTT d t₁) (liftTT d t₂)
-  | .for_all t => .for_all (liftTT d.succ t)
+/-- A Ren⋆ Δ₁ Δ₂ is a funciton that takes a typ variable and moves it
+    from the first typing context to the second --/
+@[reducible]
+def Rent (Δ₁ Δ₂ : Ctxt) : Type :=
+  ∀ {j}, (Δ₁ ∋⋆ j) → (Δ₂ ∋⋆ j)
 
-example : liftTT 0 ⋆⟪ ♯0 → ♯0 ⟫ = (⋆⟪ ♯1 → ♯1 ⟫ : 2 ⊢⋆) := rfl
-example : liftTT 1 ⋆⟪ ♯0 → ♯0 ⟫ = (⋆⟪ ♯0 → ♯0 ⟫ : 3 ⊢⋆) := rfl
-example : liftTT 1 ⋆⟪ ♯0 → ♯1 ⟫ = (⋆⟪ ♯0 → ♯2 ⟫ : 3 ⊢⋆) := rfl
-example : liftTT 0 (@polyidt 1) = (@polyidt 2)          := rfl 
+/-- lift⋆ takes a Ren⋆ and returns a different Ren⋆ that does not alter the first variable
+    but all other variables are further shifted right and have the Ren⋆ applied to the shifted-left version of them.
+    This transformation is helpful for renaming under the binders (namely ∀.) -/
+def liftt {Δ₁ Δ₂} : Rent Δ₁ Δ₂ → ∀ {k}, Rent (Δ₁ ,⋆ k) (Δ₂ ,⋆ k)
+  |  _, _, _, .here => .here
+  | rt, _, _, .there a => .there (rt a)
+ 
+/-- ren⋆ takes a Ren⋆ and a typ and applies it to that typ, moving it to the
+    new context -/
+ def rent {Δ₁ Δ₂} : Rent Δ₁ Δ₂ → ∀ {k}, Δ₁ ⊢⋆ k → Δ₂ ⊢⋆ k 
+  |  _, _, .int => .int
+  | rt, _, .var a => .var (rt a)
+  | rt, _, .arrow t₁ t₂ => .arrow (rent rt t₁) (rent rt t₂)
+  | rt, _, .prod t₁ t₂ => .prod (rent rt t₁) (rent rt t₂)
+  | rt, _, .for_all t => .for_all (rent (liftt rt) t)
 
-@[reducible] def substTT (d : Fin (n + 1)) (u : n ⊢⋆) : (n + 1) ⊢⋆ → n ⊢⋆
-  | .var ix => 
-    if h₀ : d.val = ix.val then
-      u
-    else if h₁ : ix.val >= d then by
-      cases ix
-      cases d 
-      simp at *
-      rename_i valix isLtix vald isLtd
-      unfold GE.ge at h₁
-      have a1 := Nat.lt_of_le_of_ne h₁ h₀
-      simp_arith at *
-      have a2 : vald + 1 ≤ n := Nat.le_trans a1 isLtix
-      have : n > 0 := by
-        unfold GT.gt
-        have a3 : vald < n := a2
-        exact (Nat.zero_lt_of_lt a3)
-      exact (.var (Fin.ofNat' (valix - 1) this))
-    else by
-      rw [Nat.not_ge_eq] at h₁
-      cases ix
-      cases d 
-      simp at *
-      rename_i valix isLtix vald isLtd
-      simp_arith at *
-      clear isLtix h₀
-      have w : valix + 1 ≤ n := by
-        apply Nat.le_trans
-        case m => exact vald 
-        · assumption
-        · assumption
-      simp_arith at w
-      have : n > 0 := by
-        unfold GT.gt
-        have : valix < n := w
-        exact (Nat.zero_lt_of_lt this)
-      exact (.var (Fin.ofNat' valix this))
-  | .int => .int
-  | .arrow t₁ t₂ => .arrow (substTT d u t₁) (substTT d u t₂)
-  | .prod t₁ t₂ => .prod (substTT d u t₁) (substTT d u t₂)
-  | .for_all t => .for_all (substTT d.succ (liftTT 0 u) t)
-     
-example : substTT 0 .int (⋆⟪ ♯0 → ♯0 ⟫ : 1 ⊢⋆) = ⋆⟪ int → int ⟫ := rfl
-example : substTT 1 .int (⋆⟪ ♯0 → ♯0 ⟫ : 2 ⊢⋆) = ⋆⟪ ♯0 → ♯0 ⟫ := rfl
-example : substTT 1 .int (⋆⟪ ♯0 → ♯1 ⟫ : 2 ⊢⋆) = ⋆⟪ ♯0 → int ⟫ := rfl
-example : substTT 1 ♯0 (⋆⟪ ♯0 → ♯1 ⟫ : 2 ⊢⋆) = ⋆⟪ ♯0 → ♯0 ⟫ := rfl
+/-- weaken⋆ takes a typ and returns a typ where all 
+    free typ variables in that typ have been shifted right by 1 position -/
+def weakent {Δ j k} : Δ ⊢⋆ j → Δ ,⋆ k ⊢⋆ j := rent .there
+
+theorem liftt_id : ∀ {Δ j k} {a : Δ ,⋆ k ∋⋆ j}, liftt id a = a := by
+  intros Δ j k a
+  cases a <;> simp [liftt]
+
+theorem liftt_comp : ∀ {Δ₁ Δ₂ Δ₃} {rt₁ : Rent Δ₁ Δ₂} {rt₂ : Rent Δ₂ Δ₃} {j k} {a : Δ₁ ,⋆ k ∋⋆ j},
+                     liftt (rt₂ ∘ rt₁) a = liftt rt₂ (liftt rt₁ a) := by
+  intros Δ₁ Δ₂ Δ₃ rt₁ rt₂ j k a
+  cases a <;> simp [liftt]
+
+theorem rent_id : ∀ {Δ j} {t : Δ ⊢⋆ j}, rent id t = t := by
+  intros Δ j t
+  induction t <;> try rfl
+
+  case arrow Δ' t₁ t₂ t₁_ih t₂_ih =>
+    simp [rent]
+    constructor <;> assumption
+
+  case prod Δ' t₁ t₂ t₁_ih t₂_ih =>
+    simp [rent]
+    constructor <;> assumption
+
+  case for_all Δ' j' t' t'_ih =>
+    simp [rent]
+    have : (fun {j} => @liftt Δ' Δ' id j' j) = (fun {j} => @id (Δ' ,⋆ j' ∋⋆ j)) := by
+      funext j a
+      apply liftt_id
+    rw [this]
+    assumption
+
+theorem rent_comp : ∀ {Δ₁ Δ₂ Δ₃} {rt₁ : Rent Δ₁ Δ₂} {rt₂ : Rent Δ₂ Δ₃} {j} {t : Δ₁ ⊢⋆ j},
+                    rent (rt₂ ∘ rt₁) t = rent rt₂ (rent rt₁ t) := by
+  intros Δ₁ Δ₂ Δ₃ rt₁ rt₂ j t
+  induction t generalizing Δ₂ Δ₃ rt₂ <;> try rfl
+
+  case arrow Δ' t₁ t₂ t₁_ih t₂_ih =>
+    simp [rent]
+    constructor <;> simp_all! <;> assumption
+
+  case prod Δ' t₁ t₂ t₁_ih t₂_ih =>
+    simp [rent]
+    constructor <;> simp_all! <;> assumption
+
+  case for_all Δ' k t' t'_ih =>
+    simp [rent]
+    
+    have : (fun {j} =>
+      @liftt Δ' Δ₃
+        (fun {j : Kind} => rt₂ ∘ rt₁) k j) = (fun {j} => liftt rt₂ ∘ liftt rt₁) := by 
+        funext _ t
+        apply liftt_comp
+
+    rw [this]
+    exact (@t'_ih _ _ (liftt rt₁) (liftt rt₂))
+
+theorem weakent_rent : ∀ {Δ₁ Δ₂} (rt : Rent Δ₁ Δ₂) {k} (t : Δ₁ ⊢⋆ k), 
+                        weakent (rent rt t) = rent (liftt rt (k := k)) (weakent t) := by
+  intros Δ₁ Δ₂ rt k t 
+
+  induction t generalizing Δ₂ <;> try rfl
+
+  case arrow t₁ t₂ t₁_ih t₂_ih =>
+    simp [weakent, rent]
+    constructor
+    · apply t₁_ih
+    · apply t₂_ih
+
+  case prod t₁ t₂ t₁_ih t₂_ih =>
+    simp [weakent, rent]
+    constructor
+    · apply t₁_ih
+    · apply t₂_ih
+  
+  case for_all =>
+    simp [weakent, rent] at *
+    rw [←rent_comp] at *
+    rw [←rent_comp] at *
+    congr
+    funext j'' x
+    cases x <;> rfl
+
+/-- A Subs⋆ Δ₁ Δ₂ is a function that maps typ variables to typs -/
+@[reducible]
+def Subst (Δ₁ Δ₂ : Ctxt) : Type :=
+  ∀ {j}, Δ₁ ∋⋆ j → Δ₂ ⊢⋆ j
+
+/-- lifts⋆ takes a Subs⋆ and returns a transformed Subs⋆ that does the following:
+      1. The first typ variable is unaffected (the original Subs⋆ is not applied to it)
+      2. All further variables have the Subs⋆ applied to a shift-down version of them,
+         and the but all free typ variables (that were not subs⋆ed) are brought back to their 
+         original position.
+    This transformation is helpful for substituting under the binders (namely ∀.) -/
+def liftst {Δ₁ Δ₂} : Subst Δ₁ Δ₂ → ∀ {k}, Subst (Δ₁ ,⋆ k) (Δ₂ ,⋆ k)
+  |  _, _, _, .here => .var .here
+  | st, _, _, .there a => weakent (st a)
+
+/-- subs⋆ takes a Subs⋆ and a typ and applies it to the free variables in it -/
+def subst {Δ₁ Δ₂} : Subst Δ₁ Δ₂ → ∀ {j}, Δ₁ ⊢⋆ j → Δ₂ ⊢⋆ j 
+  |  _, _, .int => .int
+  | st, _, .var a => st a
+  | st, _, .arrow t₁ t₂ => .arrow (subst st t₁) (subst st t₂)
+  | st, _, .prod t₁ t₂ => .prod (subst st t₁) (subst st t₂)
+  | st, _, .for_all t => .for_all (subst (liftst st) t)
+
+/-- extend⋆ is a Subs⋆ that, given a Subs⋆ and a typ, replaces the first free typ var with
+    that typ and applies the the given substitution to a shifted-down version of all further typ vars -/
+def extendt {Δ₁ Δ₂} : Subst Δ₁ Δ₂ → ∀ {k}, (Δ₂ ⊢⋆ k) → Subst (Δ₁ ,⋆ k) Δ₂
+  |  _, _, t, _, .here => t
+  | st, _, _, _, .there a => st a
+
+macro b:term:80 "[" a:term:80 "]⋆" : term => `(subst (extendt .var $a) $b)
+
+example : ⋆⟪ ♯0 → ♯0 ⟫[.int]⋆ = (⋆⟪ int → int ⟫ : Typ Ø ⋆) := rfl
+
+theorem subst_id : ∀ {Δ j} (t : Δ ⊢⋆ j), subst .var t = t := by
+  intros Δ j t 
+  induction t <;> 
+    try rfl 
+
+  case arrow =>
+    simp_all!
+
+  case prod =>
+    simp_all!
+
+  case for_all Δ' k t' t'_ih =>
+    simp_all!
+    have : (fun {j} => @liftst Δ' Δ' Typ.var k j) = (fun {j} => @Typ.var (Δ' ,⋆ k) j) := by
+          funext _ t
+          cases t <;> rfl
+    rw [this]
+    assumption
+
+theorem subst_var : ∀ {Δ₁ Δ₂} {st : Subst Δ₁ Δ₂} {j} (x : Δ₁ ∋⋆ j), 
+                subst st (.var x) = st x := by intros; rfl
+
+theorem weakent_subst : ∀ {Δ₁ Δ₂} (st : Subst Δ₁ Δ₂) {k} (t : Δ₁ ⊢⋆ k),
+                        weakent (subst st t) = subst (liftst st (k := k)) (weakent t) := by 
+  intros Δ₁ Δ₂ st k t 
+
+  induction t generalizing Δ₂ <;> try rfl
+
+  case arrow Δ' t₁ t₂ t₁_ih t₂_ih => 
+    simp [weakent, rent, subst]
+    constructor
+    · apply t₁_ih
+    · apply t₂_ih
+
+  case prod Δ' t₁ t₂ t₁_ih t₂_ih => 
+    simp [weakent, rent, subst]
+    constructor
+    · apply t₁_ih
+    · apply t₂_ih
+
+  case for_all Δ' j' t' t'_ih =>
+    simp [weakent, rent, subst] at *
+    generalize hs : (subst (fun {j} => liftst fun {j} => st) t') = ts
+    admit
+    /- cases ts <;>
+      cases ht' : t' <;> rw [ht'] at hs <;> simp [subst] at hs <;> try contradiction
+    · simp [subst, rent] at *
+      rename_i x x'
+      cases x'
+      · simp [liftst] at hs
+        rw [←hs]
+        rfl
+      · simp [liftst, weakent] at hs 
+        rename_i x''
+        cases hx : st x'' <;>
+          rw [hx] at hs <;> simp [rent] at hs <;> try contradiction
+        rw [←hs]
+        simp [liftt, liftst, weakent]
+        rw [hx]
+        rfl
+    · simp [liftst] at hs 
+      rename_i x
+      cases x <;> try contradiction
+      simp at hs
+      simp [weakent] at hs
+      rename_i x''
+      cases hx : st x'' <;>
+          rw [hx] at hs <;> simp [rent] at hs <;> try contradiction
+      simp [subst, rent, liftt, liftst]
+      rw [hx]
+      rfl
+    · rfl
+    ·  -/
+
+      
+
+      
+      
+      
 
 
-theorem liftTT_liftTT : ∀ n n' k (t : k ⊢⋆), 
-  liftTT n (liftTT (n + n') t) =
-  liftTT (1 + (n + n')) (liftTT n t) := by
-  intros n n' k t
-  unfold liftTT
-  admit
+      
+      
+    /- · simp_all!
+      simp [weakent, rent] -/
+
+theorem subst_comp : ∀ {Δ₁ Δ₂ Δ₃} {st₁ : Subst Δ₁ Δ₂} {st₂ : Subst Δ₂ Δ₃} {j} (t : Δ₁ ⊢⋆ j),
+               subst (subst st₂ ∘ st₁) t = subst st₂ (subst st₁ t) := by
+  intros Δ₁ Δ₂ Δ₃ st₁ st₂ j t
+  induction t generalizing Δ₂ Δ₃ <;> try rfl 
+
+  case arrow Δ' t₁ t₂ t₁_ih t₂_ih =>
+    simp [subst]
+    constructor 
+    · apply t₁_ih
+    · apply t₂_ih
+
+  case prod Δ' t₁ t₂ t₁_ih t₂_ih =>
+    simp [subst]
+    constructor 
+    · apply t₁_ih
+    · apply t₂_ih
+   
+  case for_all Δ' j' t' t'_ih =>
+    simp [subst]
+    /- set_option pp.all true in
+    rfl -/
+    have : (fun {j} => @liftst Δ' Δ₃ (fun {j} => (subst fun {j} => st₂) ∘ st₁) j' j) = (fun {j} => subst (liftst st₂) ∘ liftst st₁) := by 
+      funext _ x
+      cases x
+      · simp_all!
+      · simp_all!
+        apply weakent_subst
+      
+    rw [this]
+    simp_all!
 
