TypedAssembly.lean
@@ -2,4 +2,3 @@
 -- Import modules here that should be built as part of the library.
 import «TypedAssembly».Basic
 import «TypedAssembly».SystemF
-import «TypedAssembly».Util
