TypedAssembly/SystemF/Kind.lean
@@ -1,0 +1,9 @@
+
+inductive Kind where
+  | star
+  deriving BEq, DecidableEq, Repr
+
+namespace Kind 
+  notation "⋆" => Kind.star
+end Kind
+open Kind
