TypedAssembly/SystemF/TypeEq.lean
@@ -1,0 +1,2 @@
+import «TypedAssembly».SystemF.Typ
+
